equational_theories/Definability/Prn_prn13h12a.lean
@@ -1,0 +1,41 @@
+import equational_theories.Definability.Prn_prn13h12a_data
+
+/-! # The data lemmas for the group of order 12 on Fin 13 -/
+
+set_option maxHeartbeats 1000000
+
+open Law Law.MagmaLaw
+
+namespace prn13h12a
+
+theorem hl : ∀ i, Function.LeftInverse (Einv i) (E i) := by decide
+
+theorem hr : ∀ i, Function.RightInverse (Einv i) (E i) := by decide
+
+theorem htr : ∀ x y, E (tr x y).2 (rep (tr x y).1).1 = x ∧
+    E (tr x y).2 (rep (tr x y).1).2 = y := by decide
+
+end prn13h12a
+
+namespace prn13h12a
+
+theorem hz : ∀ i, tr (rep i).1 (rep i).2 = (i, z i) := by decide
+
+theorem hst : ∀ i j, tr (E j (rep i).1) (E j (rep i).2) = (i, st i j) := by decide
+
+end prn13h12a
+
+theorem prn13h12aM467_models : @satisfies _ (Fin 13) prn13h12aM467 Law467 :=
+  (@Law467.models_iff (Fin 13) prn13h12aM467).mpr (by native_decide)
+
+theorem prn13h12aM467_endo : ∀ i, prn13h12aM467.IsEndo (prn13h12a.E i) := by decide
+
+theorem prn13h12aM704_models : @satisfies _ (Fin 13) prn13h12aM704 Law704 :=
+  (@Law704.models_iff (Fin 13) prn13h12aM704).mpr (by native_decide)
+
+theorem prn13h12aM704_endo : ∀ i, prn13h12aM704.IsEndo (prn13h12a.E i) := by decide
+
+theorem prn13h12aM1516_models : @satisfies _ (Fin 13) prn13h12aM1516 Law1516 :=
+  (@Law1516.models_iff (Fin 13) prn13h12aM1516).mpr (by native_decide)
+
+theorem prn13h12aM1516_endo : ∀ i, prn13h12aM1516.IsEndo (prn13h12a.E i) := by decide
