equational_theories/Definability/Prn_prn8h4b.lean
@@ -25,22 +25,47 @@ theorem hst : ∀ i j, tr (E j (rep i).1) (E j (rep i).2) = (i, st i j) := by de
 
 end prn8h4b
 
-theorem prn8h4bM167_models : @satisfies _ (Fin 8) prn8h4bM167 Law167 :=
-  (@Law167.models_iff (Fin 8) prn8h4bM167).mpr (by native_decide)
+theorem prn8h4bM14_models : @satisfies _ (Fin 8) prn8h4bM14 Law14 :=
+  (@Law14.models_iff (Fin 8) prn8h4bM14).mpr (by native_decide)
 
-theorem prn8h4bM167_endo : ∀ i, prn8h4bM167.IsEndo (prn8h4b.E i) := by decide
+theorem prn8h4bM14_endo : ∀ i, prn8h4bM14.IsEndo (prn8h4b.E i) := by decide
 
-theorem prn8h4bM1483_models : @satisfies _ (Fin 8) prn8h4bM1483 Law1483 :=
-  (@Law1483.models_iff (Fin 8) prn8h4bM1483).mpr (by native_decide)
+theorem prn8h4bM477_models : @satisfies _ (Fin 8) prn8h4bM477 Law477 :=
+  (@Law477.models_iff (Fin 8) prn8h4bM477).mpr (by native_decide)
 
-theorem prn8h4bM1483_endo : ∀ i, prn8h4bM1483.IsEndo (prn8h4b.E i) := by decide
+theorem prn8h4bM477_endo : ∀ i, prn8h4bM477.IsEndo (prn8h4b.E i) := by decide
 
-theorem prn8h4bM1682_models : @satisfies _ (Fin 8) prn8h4bM1682 Law1682 :=
-  (@Law1682.models_iff (Fin 8) prn8h4bM1682).mpr (by native_decide)
+theorem prn8h4bM680_models : @satisfies _ (Fin 8) prn8h4bM680 Law680 :=
+  (@Law680.models_iff (Fin 8) prn8h4bM680).mpr (by native_decide)
 
-theorem prn8h4bM1682_endo : ∀ i, prn8h4bM1682.IsEndo (prn8h4b.E i) := by decide
+theorem prn8h4bM680_endo : ∀ i, prn8h4bM680.IsEndo (prn8h4b.E i) := by decide
 
-theorem prn8h4bM3675_models : @satisfies _ (Fin 8) prn8h4bM3675 Law3675 :=
-  (@Law3675.models_iff (Fin 8) prn8h4bM3675).mpr (by native_decide)
+theorem prn8h4bM692_models : @satisfies _ (Fin 8) prn8h4bM692 Law692 :=
+  (@Law692.models_iff (Fin 8) prn8h4bM692).mpr (by native_decide)
 
-theorem prn8h4bM3675_endo : ∀ i, prn8h4bM3675.IsEndo (prn8h4b.E i) := by decide
+theorem prn8h4bM692_endo : ∀ i, prn8h4bM692.IsEndo (prn8h4b.E i) := by decide
+
+theorem prn8h4bM1276_models : @satisfies _ (Fin 8) prn8h4bM1276 Law1276 :=
+  (@Law1276.models_iff (Fin 8) prn8h4bM1276).mpr (by native_decide)
+
+theorem prn8h4bM1276_endo : ∀ i, prn8h4bM1276.IsEndo (prn8h4b.E i) := by decide
+
+theorem prn8h4bM1519_models : @satisfies _ (Fin 8) prn8h4bM1519 Law1519 :=
+  (@Law1519.models_iff (Fin 8) prn8h4bM1519).mpr (by native_decide)
+
+theorem prn8h4bM1519_endo : ∀ i, prn8h4bM1519.IsEndo (prn8h4b.E i) := by decide
+
+theorem prn8h4bM3472_models : @satisfies _ (Fin 8) prn8h4bM3472 Law3472 :=
+  (@Law3472.models_iff (Fin 8) prn8h4bM3472).mpr (by native_decide)
+
+theorem prn8h4bM3472_endo : ∀ i, prn8h4bM3472.IsEndo (prn8h4b.E i) := by decide
+
+theorem prn8h4bM3588_models : @satisfies _ (Fin 8) prn8h4bM3588 Law3588 :=
+  (@Law3588.models_iff (Fin 8) prn8h4bM3588).mpr (by native_decide)
+
+theorem prn8h4bM3588_endo : ∀ i, prn8h4bM3588.IsEndo (prn8h4b.E i) := by decide
+
+theorem prn8h4bM4273_models : @satisfies _ (Fin 8) prn8h4bM4273 Law4273 :=
+  (@Law4273.models_iff (Fin 8) prn8h4bM4273).mpr (by native_decide)
+
+theorem prn8h4bM4273_endo : ∀ i, prn8h4bM4273.IsEndo (prn8h4b.E i) := by decide
