equational_theories/Definability/Prn_prn8h4c.lean
@@ -25,47 +25,7 @@ theorem hst : ∀ i j, tr (E j (rep i).1) (E j (rep i).2) = (i, st i j) := by de
 
 end prn8h4c
 
-theorem prn8h4cM14_models : @satisfies _ (Fin 8) prn8h4cM14 Law14 :=
-  (@Law14.models_iff (Fin 8) prn8h4cM14).mpr (by native_decide)
+theorem prn8h4cM873_models : @satisfies _ (Fin 8) prn8h4cM873 Law873 :=
+  (@Law873.models_iff (Fin 8) prn8h4cM873).mpr (by native_decide)
 
-theorem prn8h4cM14_endo : ∀ i, prn8h4cM14.IsEndo (prn8h4c.E i) := by decide
-
-theorem prn8h4cM477_models : @satisfies _ (Fin 8) prn8h4cM477 Law477 :=
-  (@Law477.models_iff (Fin 8) prn8h4cM477).mpr (by native_decide)
-
-theorem prn8h4cM477_endo : ∀ i, prn8h4cM477.IsEndo (prn8h4c.E i) := by decide
-
-theorem prn8h4cM680_models : @satisfies _ (Fin 8) prn8h4cM680 Law680 :=
-  (@Law680.models_iff (Fin 8) prn8h4cM680).mpr (by native_decide)
-
-theorem prn8h4cM680_endo : ∀ i, prn8h4cM680.IsEndo (prn8h4c.E i) := by decide
-
-theorem prn8h4cM692_models : @satisfies _ (Fin 8) prn8h4cM692 Law692 :=
-  (@Law692.models_iff (Fin 8) prn8h4cM692).mpr (by native_decide)
-
-theorem prn8h4cM692_endo : ∀ i, prn8h4cM692.IsEndo (prn8h4c.E i) := by decide
-
-theorem prn8h4cM1276_models : @satisfies _ (Fin 8) prn8h4cM1276 Law1276 :=
-  (@Law1276.models_iff (Fin 8) prn8h4cM1276).mpr (by native_decide)
-
-theorem prn8h4cM1276_endo : ∀ i, prn8h4cM1276.IsEndo (prn8h4c.E i) := by decide
-
-theorem prn8h4cM1519_models : @satisfies _ (Fin 8) prn8h4cM1519 Law1519 :=
-  (@Law1519.models_iff (Fin 8) prn8h4cM1519).mpr (by native_decide)
-
-theorem prn8h4cM1519_endo : ∀ i, prn8h4cM1519.IsEndo (prn8h4c.E i) := by decide
-
-theorem prn8h4cM3472_models : @satisfies _ (Fin 8) prn8h4cM3472 Law3472 :=
-  (@Law3472.models_iff (Fin 8) prn8h4cM3472).mpr (by native_decide)
-
-theorem prn8h4cM3472_endo : ∀ i, prn8h4cM3472.IsEndo (prn8h4c.E i) := by decide
-
-theorem prn8h4cM3588_models : @satisfies _ (Fin 8) prn8h4cM3588 Law3588 :=
-  (@Law3588.models_iff (Fin 8) prn8h4cM3588).mpr (by native_decide)
-
-theorem prn8h4cM3588_endo : ∀ i, prn8h4cM3588.IsEndo (prn8h4c.E i) := by decide
-
-theorem prn8h4cM4273_models : @satisfies _ (Fin 8) prn8h4cM4273 Law4273 :=
-  (@Law4273.models_iff (Fin 8) prn8h4cM4273).mpr (by native_decide)
-
-theorem prn8h4cM4273_endo : ∀ i, prn8h4cM4273.IsEndo (prn8h4c.E i) := by decide
+theorem prn8h4cM873_endo : ∀ i, prn8h4cM873.IsEndo (prn8h4c.E i) := by decide
